Remove generated definitions from Revm links

RocqOfRust/revm/revm_context_interface/links/journaled_state.v
@@ -212,49 +212,52 @@ Module Eip7702CodeLoad.
 End Eip7702CodeLoad.
 Export (hints) Eip7702CodeLoad.
 
-Module Impl_Eip7702CodeLoad.
+Module Impl_Deref_for_Eip7702CodeLoad.
   Definition Self (T : Set) : Set :=
     Eip7702CodeLoad.t T.
 
-  Definition into_components {T : Set} `{Link T} (self : Self T) : PolymorphicFunction.t :=
-    fun _ _ args =>
-      match args with
-      | [_] =>
-          LowM.Pure (inl (φ (
-            self.(Eip7702CodeLoad.state_load).(StateLoad.data),
-            {|
-              Eip7702CodeLoad.state_load := {|
-                StateLoad.data := tt;
-                StateLoad.is_cold :=
-                  self.(Eip7702CodeLoad.state_load).(StateLoad.is_cold);
-              |};
-              Eip7702CodeLoad.is_delegate_account_cold :=
-                self.(Eip7702CodeLoad.is_delegate_account_cold);
-            |}
-          )))
-      | _ => M.impossible "wrong number of arguments"
-      end.
-
-  Instance run_into_components {T : Set} `{Link T} (self : Self T) :
+  Instance run_deref (T : Set) `{Link T} (self : '& (Self T)) :
     Run.Trait
-      (into_components self)
-      [] [] [φ self] (T * Self unit).
+      (journaled_state.Impl_core_ops_deref_Deref_for_revm_context_interface_journaled_state_Eip7702CodeLoad_T.deref (Φ T))
+      [] [] [ φ self ] ('& (StateLoad.t T)).
   Proof.
     constructor.
-    cbn.
-    eapply Run.PureSuccess with (value := (
-      self.(Eip7702CodeLoad.state_load).(StateLoad.data),
-      {|
-        Eip7702CodeLoad.state_load := {|
-          StateLoad.data := tt;
-          StateLoad.is_cold :=
-            self.(Eip7702CodeLoad.state_load).(StateLoad.is_cold);
-        |};
-        Eip7702CodeLoad.is_delegate_account_cold :=
-          self.(Eip7702CodeLoad.is_delegate_account_cold);
-      |}
-    )).
-    reflexivity.
+    run_symbolic.
+  Defined.
+  Global Opaque run_deref.
+
+  Instance method_deref (T : Set) `{Link T} : Deref.Method_deref (Self T) (StateLoad.t T).
+  Proof.
+    econstructor.
+    { constructor.
+      eapply IsTraitMethod.Defined.
+      { apply journaled_state.Impl_core_ops_deref_Deref_for_revm_context_interface_journaled_state_Eip7702CodeLoad_T.Implements. }
+      { reflexivity. }
+    }
+    { typeclasses eauto. }
+  Defined.
+
+  Instance run (T : Set) `{Link T} : Deref.Run (Self T) (StateLoad.t T) :=
+  {}.
+End Impl_Deref_for_Eip7702CodeLoad.
+Export (hints) Impl_Deref_for_Eip7702CodeLoad.
+
+Module Impl_Eip7702CodeLoad.
+  Definition Self (T : Set) `{Link T} : Set :=
+    Eip7702CodeLoad.t T.
+
+  (* pub fn into_components(self) -> (T, Eip7702CodeLoad<()>) *)
+  Instance run_into_components (T : Set) `{Link T} (self : Self T) :
+    Run.Trait
+      (journaled_state.Impl_revm_context_interface_journaled_state_Eip7702CodeLoad_T.into_components (Φ T))
+      [] [] [ φ self ] (T * Self unit).
+  Proof.
+    constructor.
+    run_symbolic.
+    eapply Run.CallPrimitiveGetTraitMethod. {
+      apply Impl_Deref_for_Eip7702CodeLoad.method_deref.
+    }
+    run_symbolic.
   Defined.
   Global Opaque run_into_components.
 End Impl_Eip7702CodeLoad.
