RocqOfRust/revm/revm_interpreter/instructions/links/contract/extstaticcall.v
@@ -49,19 +49,6 @@ pub fn extstaticcall<WIRE: InterpreterTypes, H: Host + ?Sized>(
     host: &mut H,
 )
 *)
-Definition extstaticcall
-    {WIRE H : Set} `{Link WIRE} `{Link H}
-    {WIRE_types : InterpreterTypes.Types.t} `{InterpreterTypes.Types.AreLinks WIRE_types}
-    {H_types : Host.Types.t} `{Host.Types.AreLinks H_types}
-    (interpreter : '&mut (Interpreter.t WIRE WIRE_types))
-    (host : '&mut H) :
-    PolymorphicFunction.t :=
-  fun _ _ args =>
-    match args with
-    | [_; _] => LowM.Pure (inl (φ tt))
-    | _ => M.impossible "wrong number of arguments"
-    end.
-
 Instance run_extstaticcall
   {WIRE H : Set} `{Link WIRE} `{Link H}
   {WIRE_types : InterpreterTypes.Types.t} `{InterpreterTypes.Types.AreLinks WIRE_types}
@@ -71,12 +58,14 @@ Instance run_extstaticcall
   (interpreter : '&mut (Interpreter.t WIRE WIRE_types))
   (host : '&mut H) :
   Run.Trait
-    (extstaticcall interpreter host) [] [ Φ WIRE; Φ H ] [ φ interpreter; φ host ]
+    instructions.contract.extstaticcall [] [ Φ WIRE; Φ H ] [ φ interpreter; φ host ]
     unit.
 Proof.
   constructor.
-  cbn.
-  eapply Run.PureSuccess with (value := tt).
-  reflexivity.
+  destruct run_InterpreterTypes_for_WIRE eqn:?.
+  destruct run_LoopControl_for_Control.
+  destruct run_InputsTrait_for_Input.
+  destruct run_RuntimeFlag_for_RuntimeFlag.
+  run_symbolic.
 Defined.
 Global Opaque run_extstaticcall.
